Mlir/Printer.lean
@@ -24,60 +24,59 @@ def printIndent (identFactor: Nat) : IO Unit :=
     IO.print ("  ")
     printIndent identFactor'
 
-def printValue (ctx : IRContext) (value : ValuePtr) (hval : value.InBounds ctx := by grind) (hx : ctx.FieldsInBounds := by grind) : IO Unit := do
+def printValue (ctx : IRContext) (value : ValuePtr) : IO Unit := do
   match value with
   | ValuePtr.opResult opResultPtr =>
-    let opResult := opResultPtr.get ctx (by grind)
-    let opStruct := opResult.owner.get ctx (by grind)
+    let opResult := opResultPtr.get! ctx
+    let opStruct := opResult.owner.get! ctx
     if opStruct.results.size = 1 then
       IO.print s!"%{opResult.owner}"
     else
       IO.print s!"%{opResult.owner}_{opResult.index}"
   | ValuePtr.blockArgument blockArgPtr =>
-    let blockArg := blockArgPtr.get ctx (by grind)
+    let blockArg := blockArgPtr.get! ctx
     IO.print s!"%arg{blockArg.owner}_{blockArg.index}"
 
-def printOpResult (ctx: IRContext) (result: OpResultPtr) (hres : result.InBounds ctx := by grind) (hx : ctx.FieldsInBounds := by grind) : IO Unit := do
-  printValue ctx (ValuePtr.opResult result) (by grind) hx
+def printOpResult (ctx: IRContext) (result: OpResultPtr) : IO Unit := do
+  printValue ctx (ValuePtr.opResult result)
 
-def printOpResults (ctx: IRContext) (op: OperationPtr) (hop : op.InBounds ctx := by grind) (hx : ctx.FieldsInBounds := by grind) : IO Unit := do
-  let opStruct := op.get ctx (by grind)
-  if h : op.getNumResults! ctx ≠ 0 then
+def printOpResults (ctx: IRContext) (op: OperationPtr) : IO Unit := do
+  if op.getNumResults! ctx ≠ 0 then
     let res := op.getResult 0
     printValue ctx res
-    for h : index in 1...(op.getNumResults! ctx) do
+    for index in 1...(op.getNumResults! ctx) do
       IO.print ", "
       let res := op.getResult index
       printValue ctx res
     IO.print " = "
 
-def printOpOperands (ctx: IRContext) (op: OperationPtr) (hop : op.InBounds ctx := by grind) (hx : ctx.FieldsInBounds := by grind) : IO Unit := do
-  let opStruct := op.get ctx (by grind)
+def printOpOperands (ctx: IRContext) (op: OperationPtr) : IO Unit := do
+  let opStruct := op.get! ctx
   IO.print "("
   if h : op.getNumOperands! ctx ≠ 0 then
-    printValue ctx (op.getOperand ctx 0)
+    printValue ctx (op.getOperand! ctx 0)
     for h : index in 1...(op.getNumOperands! ctx) do
       IO.print ", "
-      printValue ctx (op.getOperand ctx index)
+      printValue ctx (op.getOperand! ctx index)
   IO.print ")"
 
 mutual
-partial def printOpList (ctx: IRContext) (op: OperationPtr) (indent: Nat := 0) (hop : op.InBounds ctx := by grind) (hx : ctx.FieldsInBounds := by grind) : IO Unit := do
+partial def printOpList (ctx: IRContext) (op: OperationPtr) (indent: Nat := 0) : IO Unit := do
   printOperation ctx op indent
-  match _ : (op.get ctx).next with
+  match _ : (op.get! ctx).next with
   | some nextOp =>
     printOpList ctx nextOp indent
   | none =>
     pure ()
 
-partial def printRegion (ctx: IRContext) (region: Region) (indent: Nat := 0) (hr : region.FieldsInBounds ctx := by grind) (hx : ctx.FieldsInBounds := by grind) : IO Unit := do
+partial def printRegion (ctx: IRContext) (region: Region) (indent: Nat := 0) : IO Unit := do
   IO.println "{"
   let block := region.firstBlock
   match _ : region.firstBlock with
   | some blockPtr =>
     printIndent (indent + 1)
     IO.println s!"^{blockPtr}:"
-    let block := blockPtr.get ctx
+    let block := blockPtr.get! ctx
     match _ : block.firstOp with
     | some firstOp =>
       printOpList ctx firstOp (indent + 2)
@@ -87,14 +86,13 @@ partial def printRegion (ctx: IRContext) (region: Region) (indent: Nat := 0) (hr
     pure ()
   IO.println "}"
 
-partial def printRegions (ctx: IRContext) (op: OperationPtr) (indent: Nat := 0)
-  hop (hfib : Operation.FieldsInBounds op ctx hop := by grind) (hx : ctx.FieldsInBounds := by grind) : IO Unit := do
-  for h : regionPtr in (op.get ctx hop).regions do
-    let region := regionPtr.get ctx
+partial def printRegions (ctx: IRContext) (op: OperationPtr) (indent: Nat := 0) : IO Unit := do
+  for i in 0...(op.getNumRegions! ctx) do
+    let region := (op.getRegion! ctx i).get! ctx
     printRegion ctx region indent
 
-partial def printOperation (ctx: IRContext) (op: OperationPtr) (indent: Nat := 0) (hop : op.InBounds ctx := by grind) (hx : ctx.FieldsInBounds := by grind) : IO Unit := do
-  let opStruct := op.get ctx
+partial def printOperation (ctx: IRContext) (op: OperationPtr) (indent: Nat := 0) : IO Unit := do
+  let opStruct := op.get! ctx
   printIndent indent
   printOpResults ctx op
   IO.print (opName opStruct.opType)
@@ -102,11 +100,11 @@ partial def printOperation (ctx: IRContext) (op: OperationPtr) (indent: Nat := 0
     IO.print s!" {opStruct.properties} "
   else
     printOpOperands ctx op
-  if opStruct.regions.size > 0 then
+  if op.getNumRegions! ctx > 0 then
     IO.print " "
-    printRegions ctx op indent (by grind)
+    printRegions ctx op indent
   IO.println ""
 end
 
-partial def printModule (ctx: IRContext) (op: OperationPtr) (hop : op.InBounds ctx) (hx : ctx.FieldsInBounds) : IO Unit := do
+partial def printModule (ctx: IRContext) (op: OperationPtr) : IO Unit := do
   printOperation ctx op
